feat: Optimize Std.Concurrent.MutableMap for seq<byte> keys in Go (#5999)
#5984 fixed this datatype to be sound in Go, but at the cost of making lookups O(n) (just as they are for the built-in `map` type). This change restores the use of Go's `sync.map`, but only if enabled for maps with `bytes` (`seq<Std.BoundedInts.uint8>`) keys. This is enabled with an additional optional `bytesKeys` parameter on constructing the map. I could not see a way to express the constraint on the type parameter, so the onus is on users to not enable this incorrectly.

Source/DafnyStandardLibraries/examples/ConcurrentExamples.dfy
@@ -2,6 +2,7 @@ module ConcurrentExamples {
 
   import opened Std.Concurrent
   import opened Std.Wrappers
+  import opened Std.BoundedInts
   import opened Helpers
 
   const p1: nat -> bool := _ => true
@@ -10,7 +11,7 @@ module ConcurrentExamples {
   const p4: (Copy, nat) -> bool := (_, _) => true
   // const p5: (object?, nat) -> bool := (_, _) => true
   const p6: (string, nat) -> bool := (_, _) => true
-
+  const p7: (bytes, nat) -> bool := (_, _) => true
 
   datatype Copy = A | B
 
@@ -205,6 +206,52 @@ module ConcurrentExamples {
     mmap.Put("Hello world", 0);
     b := mmap.HasKey("Hello world");
     expect(b);
+  }
+
+  @Test
+  method TestBytes() {
+    var mmap := new MutableMap(p7);
+    var data: bytes := [0x1, 0x2, 0x3, 0x4];
+    var b := mmap.HasKey(data);
+    expect(!b);
+    mmap.Put(data, 0);
+    var dataCopy: bytes := [0x1, 0x2, 0x3, 0x4];
+    b := mmap.HasKey(dataCopy);
+    expect(b);
+  }
+
+  @Test
+  method TestBytesOptimized() {
+    var mmap := new MutableMap(p7, true);
+    var data: bytes := [0x1, 0x2, 0x3, 0x4];
+    var b := mmap.HasKey(data);
+    expect(!b);
+    var value := mmap.Get(data);
+    expect(value == None);
+
+    mmap.Put(data, 0);
+    var dataCopy: bytes := [0x1, 0x2] + [0x3, 0x4];
+    b := mmap.HasKey(dataCopy);
+    expect(b);
+
+    var data2: bytes := [0x5, 0x6];
+    mmap.Put(data2, 1);
+    value := mmap.Get(data2);
+    expect(value == Some(1));
+
+    var keys := mmap.Keys();
+    expect keys == {data, data2};
+    var values := mmap.Values();
+    expect values == {0, 1};
+    var items := mmap.Items();
+    expect items == {(data, 0), (data2, 1)};
+    var size := mmap.Size();
+    expect size == 2;
+
+    assert p7(data, 0);
+    mmap.Remove(data);
+    items := mmap.Items();
+    expect items == {(data2, 1)};
   }
 
   // does not work everywhere
